LambdaDollarToLet.v
@@ -2,10 +2,10 @@ Require Export Common.
 Require Export LambdaDollar.
 Require Export LambdaLetDollar.
 
-Reserved Notation "e ~ₑ e'" (at level 90).
-Reserved Notation "v ~ᵥ v'" (at level 90).
-Reserved Notation "j ~ⱼ j'" (at level 90).
-Reserved Notation "k ~ₖ k'" (at level 90).
+Reserved Notation "e ~ₑ e'" (at level 40).
+Reserved Notation "v ~ᵥ v'" (at level 40).
+Reserved Notation "j ~ⱼ j'" (at level 40).
+Reserved Notation "k ~ₖ k'" (at level 40).
 Inductive sim_J {A} : J A → J' A → Prop :=
 | sim_J_fun : ∀ e e', e ~ₑ e' → J_fun e ~ⱼ J_fun' e'
 | sim_J_arg : ∀ v v', v ~ᵥ v' → J_arg v ~ⱼ J_arg' v'
@@ -16,18 +16,37 @@ with sim_K {A} : K A → K' A → Prop :=
     j ~ⱼ j' → k ~ₖ k' →
     K_cons j k ~ₖ K_let' k' (plugJ' (liftJ' j') <{ 0 }>') (* J[K] ~ let x = K' in J'[0] *)
 with sim_val {A} : val A → val' A → Prop :=
-| sim_val_abs : ∀ e e', e ~ₑ e' → val_abs e ~ᵥ val_abs' e'
+| sim_val_abs : ∀ e e', tm_abs e ~ₑ tm_abs' e' → val_abs e ~ᵥ val_abs' e'
 with sim_tm {A} : tm A → tm' A → Prop :=
 | sim_var  : ∀ a,    tm_var a ~ₑ tm_var' a
 | sim_abs  : ∀ e e', e ~ₑ e' → tm_abs e ~ₑ tm_abs' e'
 | sim_s_0  : ∀ e e', e ~ₑ e' → tm_s_0 e ~ₑ tm_s_0' e'
 | sim_app  : ∀ e1 e2 e1' e2', e1 ~ₑ e1' → e2 ~ₑ e2' → tm_app e1 e2 ~ₑ tm_app' e1' e2'
 | sim_dol  : ∀ e1 e2 e1' e2', e1 ~ₑ e1' → e2 ~ₑ e2' → tm_dol e1 e2 ~ₑ tm_dol' e1' e2'
-| sim_plug : ∀ k k' e e', k ~ₖ k' → e ~ₑ e' → plugK k e ~ₑ plugK' k' e'
+(* | sim_plug : ∀ k k' e e', k ~ₖ k' → e ~ₑ e' → plugK k e ~ₑ plugK' k' e' *)
+| sim_plug : ∀ v v' k k' e e',
+    k ~ₖ k' → e ~ₑ e' →
+    (* λ x. v $ K[0] ~ λ x. v' $ K'[0] *)
+    tm_abs  (tm_dol  (lift  (val_to_tm  v )) (plugK  (liftK  k ) (tm_var  None))) ~ₑ 
+    tm_abs' (tm_dol' (lift' (val_to_tm' v')) (plugK' (liftK' k') (tm_var' None)))
 where "e ~ₑ e'" := (sim_tm  e e')
 and   "v ~ᵥ v'" := (sim_val v v')
 and   "j ~ⱼ j'" := (sim_J   j j')
 and   "k ~ₖ k'" := (sim_K   k k').
+Global Hint Constructors sim_J : core.
+Global Hint Constructors sim_K : core.
+Global Hint Constructors sim_val : core.
+Global Hint Constructors sim_tm : core.
+
+Lemma lval_sim_inv : ∀ {A} (v : val A) (e' : tm' A),
+  v ~ₑ e' → ∃ (v' : val' A), e' = v' /\ v ~ᵥ v'.
+Proof.
+  intros. destruct v. inversion H; clear H; subst.
+  exists (val_abs' e'0); auto.
+  exists (val_abs' <{ {lift' v'} $ {plugK' (liftK' k') <{ 0 }>'} }>'); split; auto.
+  constructor.
+  eapply (sim_plug v v' k k'); eassumption.
+Qed.
 
 (* v $ K[S₀ f. e] -->'* e [f := λ x. v $ K'[x]] *)
 (* Lemma aux :
